refactoring substitutions and manipulations.
- full proofs in RTac/Ctx.

theories/Lambda/ExprSubst.v
@@ -1,6 +1,7 @@
 (** This file contains generic functions for manipulating,
  ** (i.e. substituting and finding) unification variables
  **)
+Require Import Coq.Classes.Morphisms.
 Require Import ExtLib.Core.RelDec.
 Require Import ExtLib.Data.Fun.
 Require Import ExtLib.Data.Eq.
@@ -13,8 +14,10 @@ Require Import ExtLib.Tactics.
 Require Import MirrorCore.ExprI.
 Require Import MirrorCore.VariablesI.
 Require Import MirrorCore.Util.Forwardy.
-Require Import MirrorCore.Lambda.ExprD.
+Require Import MirrorCore.Util.Nat.
+
 Require Import MirrorCore.Lambda.ExprLift.
+Require Import MirrorCore.Lambda.ExprTac.
 
 Set Implicit Arguments.
 Set Strict Implicit.
@@ -33,53 +36,73 @@ Section mentionsU.
     Cases.rewrite_all_goal; intuition.
   Qed.
 
+  Lemma if_same : forall T (a : bool) (b : T),
+      (if a then b else b) = b.
+  Proof. clear. destruct a; reflexivity. Qed.
+
+  Lemma mentionsV_lift
+  : forall v e a b,
+      _mentionsV v (lift (typ := typ) (func := func) a b e) =
+      if v ?[ lt ] a then _mentionsV v e
+      else if v ?[ lt ] (a + b) then false
+           else _mentionsV (v - b) e.
+  Proof.
+    intros v e; revert v; induction e; intro v_search; simpl; intros; intuition;
+    Cases.rewrite_all_goal; repeat rewrite if_same; intuition.
+    { repeat match goal with
+               | |- context [ match ?X with _ => _ end ] => consider X
+             end; intros; auto;
+      match goal with
+        | |- ?X = ?Y =>
+          consider X; consider Y; intros; try reflexivity;
+          subst; try solve [ exfalso ; omega ]
+      end.
+      { rewrite NPeano.Nat.add_sub in H2. congruence. }
+      { assert (v_search - b + b = v_search) by omega.
+        congruence. } }
+    { clear.
+      consider (v_search ?[ lt ] a); try reflexivity.
+      consider (v_search ?[ lt ] (a + b)); reflexivity. }
+    { replace (S v_search ?[ lt ] S a)
+         with (v_search ?[ lt ] a).
+      { consider (v_search ?[ lt ] a); try reflexivity.
+        replace (S v_search ?[ lt ] (S a + b))
+           with (v_search ?[ lt ] (a + b)).
+        { consider (v_search ?[ lt ] (a + b)); try reflexivity.
+          intros. f_equal. omega. }
+        { reflexivity. } }
+      { reflexivity. } }
+  Qed.
+
 End mentionsU.
 
-Section instantiate.
+Section expr_subst.
   Variable typ : Type.
   Variable func : Type.
-  Variable lookup : uvar -> option (expr typ func).
+  Variable lookupU : uvar -> option (expr typ func).
+  Variable lookupV : var -> option (expr typ func).
 
-  Fixpoint instantiate (under : nat) (e : expr typ func) : expr typ func :=
+  Fixpoint _subst (under : nat) (e : expr typ func) : expr typ func :=
     match e with
-      | Var _
+      | Var v =>
+        match lt_rem v under with
+          | None => e
+          | Some v' => match lookupV v' with
+                         | None => e
+                         | Some e' => lift 0 under e'
+                       end
+        end
       | Inj _ => e
-      | App l r => App (instantiate under l) (instantiate under r)
-      | Abs t e => Abs t (instantiate (S under) e)
+      | App l r => App (_subst under l) (_subst under r)
+      | Abs t e => Abs t (_subst (S under) e)
       | UVar u =>
-        match lookup u with
+        match lookupU u with
           | None => UVar u
           | Some e => lift 0 under e
         end
     end.
 
-  Definition instantiates (u : uvar) : Prop :=
-    lookup u <> None /\
-    forall u' e, lookup u' = Some e ->
-                 _mentionsU u e = false.
-
-  Lemma instantiate_instantiates
-  : forall u,
-      instantiates u ->
-      forall e under,
-        _mentionsU u (instantiate under e) = false.
-  Proof.
-    induction e; simpl; intros; auto.
-    { rewrite IHe1. auto. }
-    { destruct H.
-      consider (u ?[ eq ] u0).
-      { intros; subst.
-        specialize (H0 u0).
-        destruct (lookup u0).
-        { rewrite mentionsU_lift. auto. }
-        { congruence. } }
-      { intros.
-        consider (lookup u0); intros.
-        { rewrite mentionsU_lift. eauto. }
-        { simpl. consider (EqNat.beq_nat u u0); try congruence. } } }
-  Qed.
-
-End instantiate.
+End expr_subst.
 
 Section instantiate_thm.
   Variable typ : Type.
@@ -93,6 +116,442 @@ Section instantiate_thm.
   Context {Typ2Ok_Fun : Typ2Ok Typ2_Fun}.
   Context {RSymOk_func : RSymOk RSym_func}.
 
+  Theorem expr_subst_sound
+  : expr_subst_spec_ho
+      (fun us vs e t => ExprDsimul.ExprDenote.exprD' us vs t e)
+      (@_subst typ func).
+  Proof.
+    (** exprD'_ind does not seem powerful enough for this **)
+    red. intros. subst n. generalize dependent _tvs. revert e'. revert t.
+    induction e; simpl; intros.
+    { clear H_substU.
+      generalize (lt_rem_sound (length _tvs) v).
+      consider (lt_rem v (length _tvs)); intros.
+      { specialize (H_substV n).
+        destruct (substV n).
+        { autorewrite with exprD_rw in H1. simpl in *.
+          forward. inv_all; subst.
+          eapply nth_error_get_hlist_nth_appR in H3; simpl in H3.
+          { forward_reason. subst.
+            eapply H_substV in H0. forward_reason.
+            generalize (exprD'_lift tus' e nil _tvs tvs' x); simpl.
+            rewrite H0. intros; forward.
+            destruct r.
+            eexists; split; eauto.
+            revert H3. eapply exprTApR; auto.
+            eapply exprTPureR; auto.
+            clear - H6 H1.
+            intros. rewrite H1; clear H1.
+            rewrite H; clear H.
+            eapply (H6 c Hnil). }
+          { tauto. } }
+        { forward_reason; subst.
+          autorewrite with exprD_rw in *. simpl in *.
+          forward; inv_all; subst.
+          eapply nth_error_get_hlist_nth_appR in H1; simpl in H1; eauto.
+          forward_reason.
+          eapply H_substV in H0. forward_reason.
+          consider (nth_error_get_hlist_nth typD (_tvs ++ tvs') v); intros.
+          { eapply nth_error_get_hlist_nth_appR in H5; eauto.
+            forward_reason. rewrite H0 in H5.
+            inv_all; subst. destruct s; simpl in *.
+            rewrite H3. eexists; split; eauto.
+            revert H4. eapply exprTApR; auto.
+            eapply exprTPureR; auto.
+            clear - H6 H1.
+            intros. rewrite H6. rewrite H1.
+            f_equal. auto. }
+          { exfalso.
+            eapply nth_error_get_hlist_nth_None in H5.
+            eapply nth_error_get_hlist_nth_Some in H0.
+            destruct H0. simpl in *. clear - H5 x2.
+            eapply nth_error_length_lt in x2.
+            eapply nth_error_length_ge in H5.
+            rewrite app_length in H5. omega. } } }
+      { clear H_substV H. subst.
+        autorewrite with exprD_rw in *; simpl in *.
+        forward; inv_all; subst.
+        generalize (nth_error_get_hlist_nth_appL typD tvs _ H2).
+        generalize (nth_error_get_hlist_nth_appL typD tvs' _ H2).
+        intros; forward_reason. destruct x1; destruct x0; simpl in *.
+        revert H6. revert H3.
+        Cases.rewrite_all_goal. intros; inv_all; subst.
+        rewrite H1. eexists; split; eauto.
+        eapply exprTPureR; auto.
+        clear - H7 H5. intros.
+        rewrite H7. rewrite H5. reflexivity. } }
+    { clear H_substU H_substV.
+      subst. autorewrite with exprD_rw in *; simpl in *.
+      forward. eexists; split; eauto.
+      inv_all; subst.
+      eapply exprTPureR; auto. }
+    { clear H_substU H_substV.
+      subst. autorewrite with exprD_rw in H1; simpl in H1.
+      forward; inv_all; subst.
+      specialize (IHe2 _ _ _ _ H1 eq_refl); clear H1.
+      specialize (IHe1 _ _ _ _ H0 eq_refl); clear H0.
+      forward_reason.
+      autorewrite with exprD_rw. simpl.
+      erewrite ExprDsimul.ExprDenote.exprD'_typeof_expr by eauto.
+      Cases.rewrite_all_goal.
+      eexists; split; eauto.
+      revert H2. eapply exprTApR; auto.
+      revert H3. eapply exprTApR; auto.
+      eapply exprTPureR; auto.
+      unfold ExprDsimul.ExprDenote.exprT_App.
+      clear.
+      match goal with
+        | |- context [ match ?X with _ => _ end ] =>
+          destruct X
+      end.
+      intros.
+      rewrite H. rewrite H0. reflexivity. }
+    { clear H_substU H_substV.
+      subst. autorewrite with exprD_rw in *; simpl in *.
+      arrow_case_any.
+      { red in x1. subst. simpl in *.
+        autorewrite with eq_rw in *.
+        forward. inv_all. destruct r.
+        eapply IHe with (_tvs := x :: _tvs) in H2; eauto.
+        forward_reason.
+        change_rewrite H2.
+        eexists; split; eauto.
+        revert H4. eapply exprTApR; auto.
+        eapply exprTPureR; auto.
+        subst. clear.
+        match goal with
+          | |- context [ match ?X with _ => _ end ] =>
+            destruct X
+        end.
+        intros.
+        eapply functional_extensionality. intros.
+        eapply (H (Hcons (ExprDsimul.ExprDenote.Rcast_val eq_refl x2) _vs)). }
+      { congruence. } }
+    { clear H_substV.
+      specialize (H_substU u).
+      destruct (substU u).
+      { autorewrite with exprD_rw in *; simpl in *.
+        forward. inv_all; subst.
+        specialize (H_substU _ _ eq_refl).
+        forward_reason.
+        generalize (exprD'_lift tus' e nil _tvs tvs' x); simpl.
+        change_rewrite H. intros; forward.
+        destruct r.
+        eexists; split; eauto.
+        revert H0. eapply exprTApR; auto.
+        eapply exprTPureR; auto.
+        clear - H4. intros.
+        rewrite H. eapply (H4 c Hnil _vs d). }
+      { subst. autorewrite with exprD_rw in *; simpl in *.
+        forward. inv_all; subst. destruct r.
+        destruct (H_substU _ _ eq_refl); clear H_substU.
+        forward_reason. change_rewrite H.
+        rewrite H1. eexists; split; eauto.
+        revert H2. eapply exprTApR; auto.
+        eapply exprTPureR; auto. } }
+  Qed.
+
+  Lemma mentionsU_subst
+  : mentionsU_subst_spec (@_subst _ _) _mentionsU (@_mentionsV typ func).
+  Proof.
+    clear.
+    red. intros substU substV n u e; revert n; induction e.
+    { simpl. intros.
+      generalize (lt_rem_sound n v).
+      destruct (lt_rem v n); intros.
+      { forward_reason. subst.
+        consider (substV (v - n)); intros.
+        { split; intros.
+          { right. right.
+            exists (v - n). exists e.
+            rewrite mentionsU_lift in H1.
+            split; auto.
+            eapply rel_dec_eq_true; eauto with typeclass_instances.
+            clear - H.
+            eapply Minus.le_plus_minus_r. omega. }
+          { destruct H1; forward_reason; try congruence.
+            destruct H1; forward_reason; try congruence.
+            rewrite mentionsU_lift.
+            cut (x = v - n); intros; subst.
+            { congruence. }
+            { clear - H1.
+              match goal with
+                | _ : ?X = _ |- _ => consider X; intros
+              end.
+              omega. } } }
+        { simpl. split; intros; try congruence.
+          destruct H1; forward_reason; try congruence.
+          destruct H1; forward_reason; try congruence.
+          cut (x = v - n); intros; subst.
+          { congruence. }
+          { clear - H1.
+            match goal with
+              | _ : ?X = _ |- _ => consider X; intros
+            end.
+            omega. } } }
+      { simpl. split; intros; try congruence.
+        destruct H0; forward_reason; try congruence.
+        destruct H0; forward_reason; try congruence.
+        cut (n + x = v); intros; subst.
+        { clear H0. exfalso; omega. }
+        { clear - H0.
+          match goal with
+            | _ : ?X = _ |- _ => consider X; intros
+          end.
+          omega. } } }
+    { simpl; intros.
+      split; intros; try congruence.
+      destruct H; forward_reason; try congruence.
+      destruct H; forward_reason; try congruence. }
+    { simpl. intros.
+      replace (if _mentionsU u (_subst substU substV n e1)
+               then true
+               else _mentionsU u (_subst substU substV n e2))
+         with (orb (_mentionsU u (_subst substU substV n e1))
+                   (_mentionsU u (_subst substU substV n e2))).
+      { rewrite Bool.orb_true_iff.
+        rewrite IHe1; clear IHe1.
+        rewrite IHe2; clear IHe2. clear.
+        split; intro;
+        repeat match goal with
+                 | H : _ \/ _ |- _ => destruct H
+               end; forward_reason; Cases.rewrite_all_goal; eauto.
+        { right. left.
+          exists x. rewrite H. eauto. }
+        { right; right.
+          exists x. rewrite H. eauto. }
+        { left. destruct (_mentionsU u e1); auto. }
+        { right. left.
+          exists x. rewrite H.
+          destruct (_mentionsU x e1); eauto. }
+        { right. right.
+          exists x. rewrite H.
+          destruct (_mentionsV (n + x) e1); eauto. }
+        { consider (_mentionsU u e1); intros; eauto. }
+        { consider (_mentionsU x e1); [ left | right ]; right; left; eauto. }
+        { consider (_mentionsV (n + x) e1); [ left | right ]; right; right; eauto. } }
+      { destruct (_mentionsU u (_subst substU substV n e1)); auto. } }
+    { intros; simpl. rewrite IHe; clear IHe. reflexivity. }
+    { simpl. intros.
+      split; intros.
+      { consider (substU u0); intros.
+        { right. left.
+          exists u0. eexists.
+          rewrite mentionsU_lift in H0.
+          split. 2: eauto.
+          symmetry. eapply EqNat.beq_nat_refl. }
+        { left. simpl in *. split; auto.
+          symmetry in H0. eapply EqNat.beq_nat_eq in H0. subst.
+          auto. } }
+      { destruct H as [ ? | [ ? | ? ] ]; forward_reason.
+        { symmetry in H. eapply EqNat.beq_nat_eq in H. subst.
+          rewrite H0. simpl. symmetry. eapply EqNat.beq_nat_refl. }
+        { symmetry in H. eapply EqNat.beq_nat_eq in H. subst.
+          rewrite H0. rewrite mentionsU_lift. auto. }
+        { congruence. } } }
+  Qed.
+
+  Lemma lt_S_iff : forall a b, a < b <-> S a < S b.
+  Proof.
+    clear. split; intros; eauto using Lt.lt_n_S, Lt.lt_S_n.
+  Qed.
+
+  Lemma ge_S_iff : forall a b, a >= b <-> S a >= S b.
+  Proof.
+    clear. split; intros; eauto using Le.le_n_S, Le.le_S_n.
+  Qed.
+
+  Ltac learn :=
+    repeat match goal with
+             | _ : ?X = true |- _ =>
+               match X with
+                 | rel_dec _ _ => consider X; intros; subst
+               end
+           end.
+
+
+  Lemma mentionsV_subst
+(*
+  : forall (substU : uvar -> option (expr typ func)) substV n v e,
+      _mentionsV v (_subst substU substV n e) = true <->
+      (   (v < n /\ _mentionsV v e = true)
+       \/ (v >= n /\
+           (   (_mentionsV v e = true /\ substV (v-n) = None)
+            \/ (exists u' e', _mentionsU u' e = true /\
+                              substU u' = Some e' /\
+                              _mentionsV (v-n) e' = true)
+            \/ (exists v' e', _mentionsV (v'+n) e = true /\
+                              substV v' = Some e' /\
+                              _mentionsV (v-n) e' = true)))).
+*)
+  : mentionsV_subst_spec (@_subst _ _) _mentionsU (@_mentionsV typ func).
+
+  Proof.
+    clear. red.
+    intros substU substV n v_search e; revert n; revert v_search;
+    induction e; intros v_search n; intros.
+    { simpl.
+      generalize (lt_rem_sound n v).
+      destruct (lt_rem v n); intros; forward_reason; subst.
+      { consider (substV (v - n)); intros.
+        { rewrite mentionsV_lift. simpl.
+          split; intros; forward.
+          { right. split; [ omega | ].
+            right. right. do 2 eexists.
+            split; [ | split; eassumption ].
+            eapply rel_dec_eq_true. eauto with typeclass_instances.
+            clear - H.
+            rewrite Plus.plus_comm.
+            eapply Minus.le_plus_minus_r. omega. }
+          { destruct H1; forward_reason.
+            { exfalso. learn. intros; subst. omega. }
+            destruct H2 as [ ? | [ ? | ? ] ]; forward_reason.
+            { learn. congruence. }
+            { congruence. }
+            { learn. replace (x + n - n) with x in H0 by omega.
+              rewrite H3 in *. inv_all; subst. rewrite H4.
+              match goal with
+                | |- context [ if ?X then _ else _ ] => consider X; intros
+              end; auto.
+              exfalso; omega. } } }
+        { simpl. split; intros.
+          { right.
+            learn.
+            split; [ omega | ]. left; eauto. }
+          { destruct H1; forward_reason; learn; auto.
+            destruct H2 as [ ? | [ ? | ? ] ];
+              forward_reason; learn; auto; try congruence.
+            replace (x + n - n) with x in H0 by omega. congruence. } } }
+      { simpl. split; intros; learn.
+        { left; auto. }
+        { destruct H0; forward_reason; learn; auto.
+          destruct H1 as [ ? | [ ? | ? ] ];
+            forward_reason; learn; auto; try congruence.
+          exfalso; omega. } } }
+    { simpl. split; intros; try congruence.
+      destruct H; forward_reason; try congruence.
+      destruct H0 as [ ? | [ ? | ? ] ]; forward_reason; congruence. }
+    { simpl.
+      replace (if _mentionsV v_search (_subst substU substV n e1)
+               then true
+               else _mentionsV v_search (_subst substU substV n e2))
+         with (orb (_mentionsV v_search (_subst substU substV n e1))
+                   (_mentionsV v_search (_subst substU substV n e2))).
+      { rewrite Bool.orb_true_iff.
+        rewrite IHe1; clear IHe1.
+        rewrite IHe2; clear IHe2.
+        split; intros;
+        repeat match goal with
+                 | H : _ \/ _ |- _ => destruct H; forward_reason
+               end; Cases.rewrite_all_goal; eauto.
+        { right. split; auto.
+          right. left. do 2 eexists; split; [ | split; eassumption ].
+          rewrite H0. reflexivity. }
+        { right. split; auto.
+          right; right. do 2 eexists; split; [ | split; eassumption ].
+          rewrite H0. reflexivity. }
+        { left. split; auto. destruct (_mentionsV v_search e1); reflexivity. }
+        { right. split; auto.
+          left. destruct (_mentionsV v_search e1); eauto. }
+        { right. split; auto.
+          right. left. do 2 eexists; split; [ | split; eassumption ].
+          rewrite H0. destruct (_mentionsU x e1); reflexivity. }
+        { right. split; auto.
+          right. right. do 2 eexists; split; [ | split; eassumption ].
+          rewrite H0. destruct (_mentionsV (x+n) e1); reflexivity. }
+        { consider (_mentionsV v_search e1); intros.
+          { left; left; eauto. }
+          { right; left; eauto. } }
+        { consider (_mentionsV v_search e1); intros.
+          { left. right. split; eauto. }
+          { right; right; split; eauto. } }
+        { consider (_mentionsU x e1); intros.
+          { left; right; split; eauto.
+            right; left. do 2 eexists; split; [ | split; eassumption ]; eauto. }
+          { right; right; split; eauto.
+            right; left. do 2 eexists; split; [ | split; eassumption ]; eauto. } }
+        { consider (_mentionsV (x + n) e1);
+          intros; [ left | right ]; right; split; eauto;
+          (right; right; do 2 eexists; split; [ | split; eassumption ]; eauto). } }
+      { destruct (_mentionsV v_search (_subst substU substV n e1)); reflexivity. } }
+    { simpl. rewrite IHe; clear IHe.
+      rewrite <- lt_S_iff.
+      rewrite <- ge_S_iff.
+      eapply or_iff_compat_l.
+      eapply and_iff_compat_l.
+      eapply or_iff_compat_l.
+      simpl.
+      split; (destruct 1; [ left | right ]); forward_reason;
+      (do 2 eexists; split; [ | split; [ eassumption | ] ]; eauto).
+      rewrite <- plus_n_Sm in *. eauto.
+      rewrite <- plus_n_Sm in *. eauto. }
+    { simpl.
+      consider (substU u); intros.
+      { rewrite mentionsV_lift. simpl in *.
+        split; intros; forward.
+        { right. split; [ omega | ].
+          right. left.
+          do 2 eexists; split; [ | split; eassumption ]; eauto.
+          symmetry. eapply EqNat.beq_nat_refl. }
+        { destruct H0; forward_reason; try congruence.
+          destruct H1 as [ ? | [ ? | ? ] ]; forward_reason; try congruence.
+          consider (EqNat.beq_nat x u); intros; subst.
+          consider (v_search ?[ lt ] n); intros; try omega.
+          congruence. } }
+      { simpl. split; intros; try congruence.
+        destruct H0; forward_reason; try congruence.
+        destruct H1 as [ ? | [ ? | ? ] ]; forward_reason; try congruence.
+        consider (EqNat.beq_nat x u); intros; subst. congruence. } }
+  Qed.
+
+  Theorem Proper_subst
+  : Proper ((eq ==> eq) ==> (eq ==> eq) ==> eq ==> eq ==> eq)%signature
+           (@_subst typ func).
+  Proof.
+    clear.
+    repeat red. intros. subst.
+    revert y1.
+    induction y2; intros; simpl; eauto.
+    { forward. erewrite H0. reflexivity. reflexivity. }
+    { Cases.rewrite_all_goal. reflexivity. }
+    { rewrite IHy2. reflexivity. }
+    { erewrite H; reflexivity. }
+  Qed.
+
+  Theorem _subst_noop
+  : forall (substU : ExprI.uvar -> option (expr typ func))
+           (substV : ExprI.var -> option (expr typ func))
+     (n : nat) (e : expr typ func),
+      (forall u : ExprI.uvar, _mentionsU u e = true -> substU u = None) ->
+      (forall v : ExprI.var, _mentionsV (v+n) e = true -> substV v = None) ->
+      _subst substU substV n e = e.
+  Proof.
+    intros substU substV n e; revert n; induction e; simpl; eauto.
+    { intros.
+      generalize (lt_rem_sound n v).
+      destruct (lt_rem v n); intros; forward_reason; subst.
+      { rewrite H0. reflexivity.
+        eapply EqNat.beq_nat_true_iff. omega. }
+      { reflexivity. } }
+    { simpl; intros.
+      rewrite IHe1; clear IHe1.
+      rewrite IHe2; clear IHe2.
+      reflexivity.
+      { intros. eapply H. rewrite H1.
+        destruct (_mentionsU u e1); reflexivity. }
+      { intros. eapply H0. rewrite H1.
+        destruct (_mentionsV (v+n) e1); reflexivity. }
+      { intros. eapply H. rewrite H1.
+        destruct (_mentionsU u e1); reflexivity. }
+      { intros. eapply H0. rewrite H1.
+        destruct (_mentionsV (v+n) e1); reflexivity. } }
+    { intros. rewrite IHe; eauto. intros.
+      eapply H0. rewrite <- H1. f_equal. omega. }
+    { intros.
+      rewrite H. reflexivity. symmetry.
+      eapply EqNat.beq_nat_refl. }
+  Qed.
+(**
   Let Expr_expr := @Expr_expr _ _ RType_typ _ _.
   Local Existing Instance Expr_expr.
 
@@ -321,5 +780,5 @@ Section instantiate_thm.
           rewrite H.
           rewrite mentionsU_lift. assumption. } } }
   Qed.
-
+**)
 End instantiate_thm.
