theories/Lambda/ExprUnify.v
@@ -5,7 +5,7 @@ Require Import ExtLib.Data.Eq.
 Require Import ExtLib.Tactics.
 Require Import MirrorCore.SubstI.
 Require Import MirrorCore.Lambda.ExprUnify_common.
-Require Import MirrorCore.Lambda.ExprD.
+Require Import MirrorCore.Lambda.Expr.
 Require Import MirrorCore.Lambda.ExprLift.
 Require Import MirrorCore.Lambda.ExprTac.
 Require Import MirrorCore.Util.Forwardy.
