theories/Lambda/ExprUnify_common.v
@@ -3,7 +3,7 @@ Require Import ExtLib.Data.Option.
 Require Import ExtLib.Tactics.
 Require Import MirrorCore.SubstI.
 Require Import MirrorCore.UnifyI.
-Require Import MirrorCore.Lambda.ExprD.
+Require Import MirrorCore.Lambda.Expr.
 Require Import MirrorCore.Lambda.ExprVariables.
 Require Import MirrorCore.Lambda.ExprLift.
 Require Import MirrorCore.Lambda.ExprTac.
@@ -27,7 +27,7 @@ Section typed.
   Context {SubstUpdate_subst : SubstUpdate subst (expr typ func)}.
   Context {SubstOk_subst : SubstOk Subst_subst}.
   Context {SubstUpdateOk_subst
-  : @SubstUpdateOk _ _ _ _ Expr_expr _ _ SubstUpdate_subst _}.
+  : @SubstUpdateOk _ _ _ _ (Expr_expr _ _ _ _) _ SubstUpdate_subst _}.
 
   Lemma handle_set
   : forall (e0 : expr typ func) (u : uvar) (s s' : subst)
