theories/RTac/CoreK.v
@@ -30,12 +30,6 @@ Section parameterized.
   Context {Typ0_Prop : Typ0 _ Prop}.
   Context {Expr_expr : Expr RType_typ expr}.
   Context {ExprOk_expr : ExprOk Expr_expr}.
-  Context {ExprVar_expr : ExprVar expr}.
-  Context {ExprVarOk_expr : ExprVarOk _}.
-  Context {ExprUVar_expr : ExprUVar expr}.
-  Context {ExprUVarOk_expr : ExprUVarOk _}.
-  Context {MentionsAny_expr : MentionsAny expr}.
-  Context {MentionsAnyOk_expr : MentionsAnyOk _ _ _}.
 
 (*
   (** TODO(gmalecha): These should go somewhere more useful *)
@@ -111,7 +105,7 @@ Section parameterized.
 
   Theorem Proper_rtacK_spec ctx s
   : Proper (EqGoal (getUVars ctx) (getVars ctx) ==>
-            @EqResult _ _ _ _ _ _ ctx ==> iff)
+            @EqResult _ _ _ _ _ ctx ==> iff)
            (@rtacK_spec ctx s).
   Proof.
     red. red. red.
@@ -178,7 +172,7 @@ Section parameterized.
 
 End parameterized.
 
-Arguments rtacK_sound {typ expr _ _ _ _} tac : rename.
+Arguments rtacK_sound {typ expr _ _ _} tac : rename.
 
 Export MirrorCore.ExprI.
 Export MirrorCore.SubstI.
